.

coq_proofs/borrowing_calculus/proofs/expr.v
@@ -1,6 +1,6 @@
 Require Import String ZArith Coq.FSets.FMapAVL Coq.Structures.OrderedTypeEx.
 Require Import Coq.FSets.FSetProperties Coq.FSets.FMapFacts FMaps FSetAVL Nat PeanoNat.
-Require Import Coq.Arith.EqNat Coq.ZArith.Int Integers types.
+Require Import Coq.Arith.EqNat Coq.ZArith.Int Integers type.
 
 Set Implicit Arguments.
 Unset Strict Implicit.
@@ -16,15 +16,26 @@ Inductive expr : Type :=
 | Cons : ident -> list expr -> expr
 | Match : quantity -> expr -> list ((ident * list ident) * expr) -> expr.
 
-(* Typing rules *)
+(* Typing rules *) 
 Inductive type_expr : typing_context -> expr -> (quantity * type) -> typing_context -> Prop :=
 | Ty_var_lin : forall Gamma x t,
               type_expr (extend_context Gamma x (Lin, t)) (Var x) (Lin, t) Gamma
 | Ty_var_un : forall Gamma x t,
               type_expr (extend_context Gamma x (Un, t)) (Var x) (Un, t) (extend_context Gamma x (Un, t))
 | Ty_var_bor : forall Gamma x t,
-              type_expr (extend_context Gamma x (Bor, t)) (Var x) (Bor, t) (extend_context Gamma x (Bor, t)).
-(* weakening: adding extra, unneeded assumptions to the typing context does not prevent the expr from type checking *)
+               type_expr (extend_context Gamma x (Bor, t)) (Var x) (Bor, t) (extend_context Gamma x (Bor, t))
+(* unrestricted variable can be used linearly or borrowed freely *)
+| Ty_var_un_bor_lin : forall Gamma x q t,
+                      List.In q (Lin :: Bor :: nil) ->
+                      type_expr (extend_context Gamma x (Un, t)) (Var x) (q, t) (extend_context Gamma x (Un, t))
+(* borrow should be only allowed in the region it is suppose to and after that it should be restored to its quantity *)
+| Ty_borrow : forall Gamma xs ts e q t Gamma', 
+              type_expr (append_only_bor Gamma xs ts) e (lift_quan q, t) (append_only_bor Gamma' xs ts) ->
+              type_expr (append_only_lin Gamma xs ts) (Borrow xs e) (q, t) (append_only_lin Gamma' xs ts).
+
+
+
+
 
 
            
