coq_proofs/borrowing_calculus/proofs/typing_proofs.v
@@ -1,3 +1,22 @@
 Require Import String ZArith Coq.FSets.FMapAVL Coq.Structures.OrderedTypeEx.
 Require Import Coq.FSets.FSetProperties Coq.FSets.FMapFacts FMaps FSetAVL Nat PeanoNat.
-Require Import Coq.Arith.EqNat Coq.ZArith.Int Integers type.
+Require Import Coq.Arith.EqNat Coq.ZArith.Int Integers type expr.
+
+Set Implicit Arguments.
+Unset Strict Implicit.
+Unset Printing Implicit Defensive.
+
+(* add assumption about transposition related to equality of Gamma3 and Gamma3' *)
+Lemma exchange : forall Gamma1 x1 t1 x2 t2 Gamma2 e t Gamma3 Gamma3',
+type_expr (append_context (extend_context (extend_context Gamma1 x1 t1) x2 t2) Gamma2) e t Gamma3 ->
+type_expr (append_context (extend_context (extend_context Gamma1 x2 t2) x1 t1) Gamma2) e t Gamma3'.
+Proof.
+Admitted.
+
+
+(* weakening: adding extra, unneeded assumptions to the typing context does not prevent the expr from type checking *)
+Lemma weakening: forall Gamma e T Gamma' x T',
+type_expr Gamma e T Gamma' ->
+type_expr (extend_context Gamma x T') e T (extend_context Gamma' x T').
+Proof.
+Admitted.
